Introduce Hoare triples

heaplang/base.v
@@ -54,8 +54,99 @@ Proof.
   (* Now we are left with a trivial proof that 1+2 = 3 *)
   done.
 Qed.
-End heaplang.
 
 (*
   The full list of evaluation tactics can be found at https://gitlab.mpi-sws.org/iris/iris/-/blob/master/docs/heap_lang.md
 *)
+
+(*
+  Let's use this knowledge to prove a specification for a larger program
+*)
+Lemma wp_prog_add_2 : ⊢ WP prog + #2 {{v, ⌜v = #5⌝}}.
+Proof.
+  iStartProof.
+  (*
+    The first part of this program is to evaluate `prog`. So we can seperate the program into 2 parts.
+    First we evaluate `prog`, then we take the result and add 2 to it.
+    To do this we can use `wp_bind`.
+  *)
+  wp_bind prog.
+  (*
+    Now we have the problem that our post condition doesn't match the one we proved.
+    To fix this we can use monitonicity of WP.
+  *)
+  iApply wp_mono.
+  2: { iApply wp_prog. }
+  iIntros "%_ ->".
+  (* And now we can evaluate the rest of the program *)
+  wp_pures.
+  (* This post condition is again trivial *)
+  done.
+Qed.
+
+(*
+  The previous proof worked, but it is not very ergonomic.
+  To fix this, we'll make `wp_prog` generic on its post condition.
+*)
+Lemma wp_prog_2 (Φ : val → iProp Σ) : (∀ v, ⌜v = #3⌝ -∗ Φ v) -∗ WP prog {{v, Φ v}}.
+Proof.
+  iIntros "HΦ".
+  rewrite /prog.
+  wp_alloc l as "Hl".
+  wp_load.
+  wp_store.
+  wp_load.
+  by iApply "HΦ".
+Qed.
+
+(* Now the other proof becomes much simpler. *)
+Lemma wp_prog_add_2_2 : ⊢ WP prog + #2 {{v, ⌜v = #5⌝}}.
+Proof.
+  wp_bind prog.
+  (* Now the proof is on the exact for required by `wp_prog_2` *)
+  iApply wp_prog_2.
+  (* And the proof proceeds as before *)
+  iIntros "%_ ->".
+  by wp_pures.
+Qed.
+
+(*
+  Hoare triples are an extended version of WP that contains a precondition.
+  They are defined as `∀ Φ, Pre -∗ (▷ ∀ r0 .. rn, Post -∗ Φ v) -∗ WP e {{v, Φ v}}`.
+  This may seem like very long and complicated definition, so let's look at it's parts.
+
+  Like before, Hoare triples are parameterised on the post conditions that are satisfied by Post. This allows us to further specialize the posible return values by specifying it as a pattern quantified over arbitrary parameters.
+  The implication of the post condition is hidden under a later, signifying that the program takes at least one step.
+  And finaly we now have a precondition.
+
+  The syntax for Hoare triples is as follows:
+  `{{{ Pre }}} e {{{ r0 .. rn, RET v; Post }}}`
+  - `Pre`: the precondiction that is assumed to hold before the program runs.
+  - `e`: the program to run.
+  - `r0 .. rn`: the parameters used to define the return value.
+  - `v`: an expression specifying the shape of the return value.
+  - `Post`: the postcondition satisfied after the program has halted.
+*)
+
+(* Let's consider a function that swaps 2 valued *)
+Definition swap : val :=
+  λ: "x" "y",
+  let: "v" := !"x" in
+  "x" <- !"y";;
+  "y" <- "v".
+
+(* To specify this program we use a Hoare triple *)
+Lemma wp_swap (l1 l2 : loc) (v1 v2 : val) : {{{l1 ↦ v1 ∗ l2 ↦ v2}}} swap #l1 #l2 {{{RET #(); l1 ↦ v2 ∗ l2 ↦ v1}}}.
+Proof.
+  iIntros "%Φ [H1 H2] HΦ".
+  rewrite /swap.
+  wp_pures.
+  wp_load.
+  wp_load.
+  wp_store.
+  wp_store.
+  iApply "HΦ".
+  by iFrame.
+Qed.
+
+End heaplang.
